vault/3-modeling/dafny/ASN-0027/modeling-1/RearrangeOps.dfy
@@ -1,0 +1,37 @@
+include "../../../../proofs/TumblerAlgebra/TumblerAlgebra.dfy"
+include "../../../../proofs/Foundation/Foundation.dfy"
+
+module RearrangeOps {
+  import opened TumblerAlgebra
+  import opened Foundation
+
+  // Shared REARRANGE operations on seq-based V-space.
+
+  // --- Cut validity predicates ---
+
+  predicate ValidPivotCuts(c1: nat, c2: nat, c3: nat, n: nat) {
+    1 <= c1 && c1 < c2 && c2 < c3 && c3 <= n + 1
+  }
+
+  predicate ValidSwapCuts(c1: nat, c2: nat, c3: nat, c4: nat, n: nat) {
+    1 <= c1 && c1 < c2 && c2 < c3 && c3 < c4 && c4 <= n + 1
+  }
+
+  // --- Concrete rearrange operations ---
+
+  // Pivot rearrange (m = 3): swaps adjacent blocks [c1,c2) and [c2,c3)
+  function PivotRearrangeV(v: seq<IAddr>, c1: nat, c2: nat, c3: nat): (v': seq<IAddr>)
+    requires ValidPivotCuts(c1, c2, c3, |v|)
+    ensures |v'| == |v|
+  {
+    v[..c1-1] + v[c2-1..c3-1] + v[c1-1..c2-1] + v[c3-1..]
+  }
+
+  // Swap rearrange (m = 4): reverses order of blocks [c1,c2), [c2,c3), [c3,c4)
+  function SwapRearrangeV(v: seq<IAddr>, c1: nat, c2: nat, c3: nat, c4: nat): (v': seq<IAddr>)
+    requires ValidSwapCuts(c1, c2, c3, c4, |v|)
+    ensures |v'| == |v|
+  {
+    v[..c1-1] + v[c3-1..c4-1] + v[c2-1..c3-1] + v[c1-1..c2-1] + v[c4-1..]
+  }
+}
